lakefile.lean
@@ -9,6 +9,9 @@ lean_lib ExtParser {
   -- add library configuration options here
 }
 
+require mathlib from git
+  "https://github.com/leanprover-community/mathlib4" @ "28c23e3c3744968baf25c65dadf7a117ec087dce"
+
 @[default_target]
 lean_exe extParser {
   root := `Main
